Rewriting.

theories/base_logic/lib/mono_list.v
@@ -15,74 +15,74 @@ Global Instance subG_mono_listΣ {A Σ} :
   subG (mono_listΣ A) Σ → (mono_listG A) Σ.
 Proof. solve_inG. Qed.
 
-Local Definition mono_list_auth_own_def `{!mono_listG A Σ}
+Local Definition mono_list_auth_def `{!mono_listG A Σ}
     (γ : gname) (q : Qp) (l : list A) : iProp Σ :=
   own γ (●ML{#q} (l : listO (leibnizO A))).
-Local Definition mono_list_auth_own_aux : seal (@mono_list_auth_own_def).
+Local Definition mono_list_auth_aux : seal (@mono_list_auth_def).
 Proof. by eexists. Qed.
-Definition mono_list_auth_own := mono_list_auth_own_aux.(unseal).
-Local Definition mono_list_auth_own_unseal :
-  @mono_list_auth_own = @mono_list_auth_own_def := mono_list_auth_own_aux.(seal_eq).
-Global Arguments mono_list_auth_own {A Σ _} γ q l.
+Definition mono_list_auth := mono_list_auth_aux.(unseal).
+Local Definition mono_list_auth_unseal :
+  @mono_list_auth = @mono_list_auth_def := mono_list_auth_aux.(seal_eq).
+Global Arguments mono_list_auth {A Σ _} γ q l.
 
-Local Definition mono_list_lb_own_def `{!mono_listG A Σ}
+Local Definition mono_list_lb_def `{!mono_listG A Σ}
     (γ : gname) (l : list A) : iProp Σ :=
   own γ (◯ML (l : listO (leibnizO A))).
-Local Definition mono_list_lb_own_aux : seal (@mono_list_lb_own_def).
+Local Definition mono_list_lb_aux : seal (@mono_list_lb_def).
 Proof. by eexists. Qed.
-Definition mono_list_lb_own := mono_list_lb_own_aux.(unseal).
-Local Definition mono_list_lb_own_unseal :
-  @mono_list_lb_own = @mono_list_lb_own_def := mono_list_lb_own_aux.(seal_eq).
-Global Arguments mono_list_lb_own {A Σ _} γ l.
+Definition mono_list_lb := mono_list_lb_aux.(unseal).
+Local Definition mono_list_lb_unseal :
+  @mono_list_lb = @mono_list_lb_def := mono_list_lb_aux.(seal_eq).
+Global Arguments mono_list_lb {A Σ _} γ l.
 
-Definition mono_list_idx_own `{!mono_listG A Σ}
+Definition mono_list_mapsto `{!mono_listG A Σ}
     (γ : gname) (i : nat) (a : A) : iProp Σ :=
-  ∃ l : list A, ⌜ l !! i = Some a ⌝ ∗ mono_list_lb_own γ l.
+  ∃ l : list A, ⌜ l !! i = Some a ⌝ ∗ mono_list_lb γ l.
 
 Local Ltac unseal := rewrite
-  /mono_list_idx_own ?mono_list_auth_own_unseal /mono_list_auth_own_def
-  ?mono_list_lb_own_unseal /mono_list_lb_own_def.
+  /mono_list_mapsto ?mono_list_auth_unseal /mono_list_auth_def
+  ?mono_list_lb_unseal /mono_list_lb_def.
 
 Section mono_list_own.
   Context `{!mono_listG A Σ}.
   Implicit Types (l : list A) (i : nat) (a : A).
 
-  Global Instance mono_list_auth_own_timeless γ q l : Timeless (mono_list_auth_own γ q l).
+  Global Instance mono_list_auth_timeless γ q l : Timeless (mono_list_auth γ q l).
   Proof. unseal. apply _. Qed.
-  Global Instance mono_list_lb_own_timeless γ l : Timeless (mono_list_lb_own γ l).
+  Global Instance mono_list_lb_timeless γ l : Timeless (mono_list_lb γ l).
   Proof. unseal. apply _. Qed.
-  Global Instance mono_list_lb_own_persistent γ l : Persistent (mono_list_lb_own γ l).
+  Global Instance mono_list_lb_persistent γ l : Persistent (mono_list_lb γ l).
   Proof. unseal. apply _. Qed.
-  Global Instance mono_list_idx_own_timeless γ i a :
-    Timeless (mono_list_idx_own γ i a) := _.
-  Global Instance mono_list_idx_own_persistent γ i a :
-    Persistent (mono_list_idx_own γ i a) := _.
+  Global Instance mono_list_mapsto_timeless γ i a :
+    Timeless (mono_list_mapsto γ i a) := _.
+  Global Instance mono_list_mapsto_persistent γ i a :
+    Persistent (mono_list_mapsto γ i a) := _.
 
-  Global Instance mono_list_auth_own_fractional γ l :
-    Fractional (λ q, mono_list_auth_own γ q l).
+  Global Instance mono_list_auth_fractional γ l :
+    Fractional (λ q, mono_list_auth γ q l).
   Proof. unseal. intros p q. by rewrite -own_op -mono_list_auth_dfrac_op. Qed.
-  Global Instance mono_list_auth_own_as_fractional γ q l :
-    AsFractional (mono_list_auth_own γ q l) (λ q, mono_list_auth_own γ q l) q.
+  Global Instance mono_list_auth_as_fractional γ q l :
+    AsFractional (mono_list_auth γ q l) (λ q, mono_list_auth γ q l) q.
   Proof. split; [auto|apply _]. Qed.
 
-  Lemma mono_list_auth_own_agree γ q1 q2 l1 l2 :
-    mono_list_auth_own γ q1 l1 -∗
-    mono_list_auth_own γ q2 l2 -∗
+  Lemma mono_list_auth_agree γ q1 q2 l1 l2 :
+    mono_list_auth γ q1 l1 -∗
+    mono_list_auth γ q2 l2 -∗
     ⌜(q1 + q2 ≤ 1)%Qp ∧ l1 = l2⌝.
   Proof.
     unseal. iIntros "H1 H2".
     by iDestruct (own_valid_2 with "H1 H2") as %?%mono_list_auth_dfrac_op_valid_L.
   Qed.
-  Lemma mono_list_auth_own_exclusive γ l1 l2 :
-    mono_list_auth_own γ 1 l1 -∗ mono_list_auth_own γ 1 l2 -∗ False.
+  Lemma mono_list_auth_exclusive γ l1 l2 :
+    mono_list_auth γ 1 l1 -∗ mono_list_auth γ 1 l2 -∗ False.
   Proof.
     iIntros "H1 H2".
-    iDestruct (mono_list_auth_own_agree with "H1 H2") as %[]; done.
+    iDestruct (mono_list_auth_agree with "H1 H2") as %[]; done.
   Qed.
 
   Lemma mono_list_auth_lb_valid γ q l1 l2 :
-    mono_list_auth_own γ q l1 -∗
-    mono_list_lb_own γ l2 -∗
+    mono_list_auth γ q l1 -∗
+    mono_list_lb γ l2 -∗
     ⌜ (q ≤ 1)%Qp ∧ l2 `prefix_of` l1 ⌝.
   Proof.
     unseal. iIntros "Hauth Hlb".
@@ -90,16 +90,16 @@ Section mono_list_own.
   Qed.
 
   Lemma mono_list_lb_valid γ l1 l2 :
-    mono_list_lb_own γ l1 -∗
-    mono_list_lb_own γ l2 -∗
+    mono_list_lb γ l1 -∗
+    mono_list_lb γ l2 -∗
     ⌜ l1 `prefix_of` l2 ∨ l2 `prefix_of` l1 ⌝.
   Proof.
     unseal. iIntros "H1 H2".
     by iDestruct (own_valid_2 with "H1 H2") as %?%mono_list_lb_op_valid_L.
   Qed.
 
-  Lemma mono_list_idx_agree γ i a1 a2 :
-    mono_list_idx_own γ i a1 -∗ mono_list_idx_own γ i a2 -∗ ⌜ a1 = a2 ⌝.
+  Lemma mono_list_mapsto_agree γ i a1 a2 :
+    mono_list_mapsto γ i a1 -∗ mono_list_mapsto γ i a2 -∗ ⌜ a1 = a2 ⌝.
   Proof.
     iDestruct 1 as (l1 Hl1) "H1". iDestruct 1 as (l2 Hl2) "H2".
     iDestruct (mono_list_lb_valid with "H1 H2") as %Hpre.
@@ -107,8 +107,8 @@ Section mono_list_own.
     destruct Hpre as [Hpre|Hpre]; eapply prefix_lookup in Hpre; eauto; congruence.
   Qed.
 
-  Lemma mono_list_auth_idx_lookup γ q l i a :
-    mono_list_auth_own γ q l -∗ mono_list_idx_own γ i a -∗ ⌜ l !! i = Some a ⌝.
+  Lemma mono_list_auth_mapsto_lookup γ q l i a :
+    mono_list_auth γ q l -∗ mono_list_mapsto γ i a -∗ ⌜ l !! i = Some a ⌝.
   Proof.
     iIntros "Hauth". iDestruct 1 as (l1 Hl1) "Hl1".
     iDestruct (mono_list_auth_lb_valid with "Hauth Hl1") as %[_ Hpre].
@@ -116,36 +116,36 @@ Section mono_list_own.
     eapply prefix_lookup in Hpre; eauto; congruence.
   Qed.
 
-  Lemma mono_list_lb_own_get γ q l :
-    mono_list_auth_own γ q l -∗ mono_list_lb_own γ l.
+  Lemma mono_list_lb_get γ q l :
+    mono_list_auth γ q l -∗ mono_list_lb γ l.
   Proof. intros. unseal. by apply own_mono, mono_list_included. Qed.
-  Lemma mono_list_lb_own_le {γ l} l' :
+  Lemma mono_list_lb_le {γ l} l' :
     l' `prefix_of` l →
-    mono_list_lb_own γ l -∗ mono_list_lb_own γ l'.
+    mono_list_lb γ l -∗ mono_list_lb γ l'.
   Proof. unseal. intros. by apply own_mono, mono_list_lb_mono. Qed.
 
-  Lemma mono_list_idx_own_get {γ l} i a :
+  Lemma mono_list_mapsto_get {γ l} i a :
     l !! i = Some a →
-    mono_list_lb_own γ l -∗ mono_list_idx_own γ i a.
+    mono_list_lb γ l -∗ mono_list_mapsto γ i a.
   Proof. iIntros (Hli) "Hl". iExists l. by iFrame. Qed.
 
-  Lemma mono_list_own_alloc l :
-    ⊢ |==> ∃ γ, mono_list_auth_own γ 1 l ∗ mono_list_lb_own γ l.
+  Lemma mono_list_alloc l :
+    ⊢ |==> ∃ γ, mono_list_auth γ 1 l ∗ mono_list_lb γ l.
   Proof.
     unseal. setoid_rewrite <- own_op. by apply own_alloc, mono_list_both_valid_L.
   Qed.
-  Lemma mono_list_auth_own_update {γ l} l' :
+  Lemma mono_list_auth_update {γ l} l' :
     l `prefix_of` l' →
-    mono_list_auth_own γ 1 l ==∗ mono_list_auth_own γ 1 l' ∗ mono_list_lb_own γ l'.
+    mono_list_auth γ 1 l ==∗ mono_list_auth γ 1 l' ∗ mono_list_lb γ l'.
   Proof.
     iIntros (?) "Hauth".
-    iAssert (mono_list_auth_own γ 1 l') with "[> Hauth]" as "Hauth".
+    iAssert (mono_list_auth γ 1 l') with "[> Hauth]" as "Hauth".
     { unseal. iApply (own_update with "Hauth"). by apply mono_list_update. }
-    iModIntro. iSplit; [done|]. by iApply mono_list_lb_own_get.
+    iModIntro. iSplit; [done|]. by iApply mono_list_lb_get.
   Qed.
 
-  Lemma mono_list_auth_own_update_app {γ l} l' :
-    mono_list_auth_own γ 1 l ==∗
-    mono_list_auth_own γ 1 (l ++ l') ∗ mono_list_lb_own γ (l ++ l').
-  Proof. by apply mono_list_auth_own_update, prefix_app_r. Qed.
+  Lemma mono_list_auth_update_app {γ l} l' :
+    mono_list_auth γ 1 l ==∗
+    mono_list_auth γ 1 (l ++ l') ∗ mono_list_lb γ (l ++ l').
+  Proof. by apply mono_list_auth_update, prefix_app_r. Qed.
 End mono_list_own.
